theories/theories/utp_designs.thy
@@ -7,70 +7,297 @@
 header {* UTP Designs *}
 
 theory utp_designs
-imports "../alpha/utp_alpha_pred" "../alpha/utp_alpha_rel" "../alpha/utp_alpha_expr"
+imports "../alpha/utp_alpha_laws" "../tactics/utp_alpha_tac" "../tactics/utp_alpha_expr_tac" utp_theory
 begin
 
-context ALPHA_PRED_BOOL
-begin
+default_sort BOOL_SORT
 
 subsection {* Constructs *}
 
-definition okay :: "'TYPE VAR" where
-"okay \<equiv> (\<lparr>name_str = ''okay'',
-         dashes = 0,
-         subscript = NoSub\<rparr>, BoolType)"
+definition "okay  \<equiv> MkVar (MkName ''okay'' 0 NoSub) BoolType True"
+definition "okay' \<equiv> MkVar (MkName ''okay'' 1 NoSub) BoolType True"
 
-definition okay' :: "'TYPE VAR" where
-"okay' \<equiv> (\<lparr>name_str = ''okay'',
-          dashes = 1,
-          subscript = NoSub\<rparr>, BoolType)"
+lemma okay_simps [simp]: 
+  "okay \<noteq> okay'" "okay' \<noteq> okay"
+  "MkBool True \<rhd> okay" "MkBool False \<rhd> okay"
+  "MkBool True \<rhd> okay'" "MkBool False \<rhd> okay'"
+  "TrueE \<rhd>\<^sub>e okay" "FalseE \<rhd>\<^sub>e okay"
+  "TrueE \<rhd>\<^sub>e okay'" "FalseE \<rhd>\<^sub>e okay'"
+  "type okay = BoolType" "type okay' = BoolType"
+  "control okay" "control okay'"
+  by (force intro:typing defined simp add:okay_def okay'_def)+
 
-abbreviation OK where "OK \<equiv> {okay,okay'}"
+abbreviation OK where "OK \<equiv> Abs_fset {okay,okay'}"
 
 abbreviation ok_true :: 
-  "('VALUE, 'TYPE) ALPHA_PREDICATE \<Rightarrow> ('VALUE, 'TYPE) ALPHA_PREDICATE" ("_\<^sup>t" [150]) where
-"p\<^sup>t \<equiv> p[true|okay]\<alpha>"
+  "'VALUE WF_ALPHA_PREDICATE \<Rightarrow> 'VALUE WF_ALPHA_PREDICATE" ("_\<^sup>t" [150]) where
+"p\<^sup>t \<equiv> p[TrueAE|okay]\<alpha>"
 
 abbreviation ok_false :: 
-  "('VALUE, 'TYPE) ALPHA_PREDICATE \<Rightarrow> ('VALUE, 'TYPE) ALPHA_PREDICATE" ("_\<^sup>f" [150]) where
-"p\<^sup>f \<equiv> p[false|okay]\<alpha>"
-
-abbreviation "ok  a \<equiv> &okay \<oplus>\<alpha> a"
-abbreviation "ok' a \<equiv> &okay' \<oplus>\<alpha> a"
+  "'VALUE WF_ALPHA_PREDICATE \<Rightarrow> 'VALUE WF_ALPHA_PREDICATE" ("_\<^sup>f" [150]) where
+"p\<^sup>f \<equiv> p[FalseAE|okay]\<alpha>"
 
 
-definition DesignD :: 
-"('VALUE, 'TYPE) ALPHA_PREDICATE \<Rightarrow>
- ('VALUE, 'TYPE) ALPHA_PREDICATE \<Rightarrow>
- ('VALUE, 'TYPE) ALPHA_PREDICATE" (infixr "\<turnstile>" 60) where
-"\<lbrakk> p \<in> WF_ALPHA_PREDICATE; q \<in> WF_ALPHA_PREDICATE; \<alpha> p = \<alpha> q \<rbrakk> \<Longrightarrow> 
-   p \<turnstile> q \<equiv> (ok (\<alpha> p) \<and>\<alpha> p) \<Rightarrow>\<alpha> (ok' (\<alpha> q) \<and>\<alpha> q)"
+abbreviation "ok  \<equiv> VarA okay"
+abbreviation "ok' \<equiv> VarA okay'"
 
+definition DesignA :: 
+"'VALUE WF_ALPHA_PREDICATE \<Rightarrow>
+ 'VALUE WF_ALPHA_PREDICATE \<Rightarrow>
+ 'VALUE WF_ALPHA_PREDICATE" (infixr "\<turnstile>" 60) where
+"p \<turnstile> q \<equiv> (ok \<and>\<alpha> p) \<Rightarrow>\<alpha> (ok' \<and>\<alpha> q)"
+
+(*
+lift_definition DesignA ::
+"'VALUE WF_ALPHA_PREDICATE \<Rightarrow>
+ 'VALUE WF_ALPHA_PREDICATE \<Rightarrow>
+ 'VALUE WF_ALPHA_PREDICATE" (infixr "\<turnstile>\<^sub>\<alpha>" 60) is
+"\<lambda> p q. (OK \<union>\<^sub>f \<alpha> p \<union>\<^sub>f \<alpha> q, \<pi> p \<turnstile> \<pi> q)" 
+  apply (auto simp add:WF_ALPHA_PREDICATE_def WF_PREDICATE_OVER_def)
+  apply (simp add:DesignP_def)
+  apply (rule unrest)
+  apply (rule unrest)
+  apply (force intro: unrest)
+  apply (force intro: unrest)
+  apply (rule unrest)
+  apply (force intro: unrest)+
+done
+*)
+
+(*
 definition SkipD ::
-"'TYPE ALPHABET \<Rightarrow> ('VALUE, 'TYPE) ALPHA_PREDICATE" ("IID") where
-"IID a = (true a \<turnstile> II\<alpha> a)"
+"'VALUE WF_PREDICATE" ("IID") where
+"IID = (true \<turnstile> II)"
+*)
 
-definition "H1 \<equiv> \<lambda> x. ok (\<alpha> x) \<Rightarrow>\<alpha> x"
+definition SkipA ::
+  "'VALUE ALPHABET \<Rightarrow> 'VALUE WF_ALPHA_PREDICATE" ("IID") where
+"IID a \<equiv> true a \<turnstile> II\<alpha> a"
 
-definition J :: "'TYPE ALPHABET \<Rightarrow> ('VALUE, 'TYPE) ALPHA_PREDICATE" where
-"J a \<equiv> (ok a \<Rightarrow>\<alpha> ok' a) \<and>\<alpha> (II\<alpha> a)"
+(*
+lift_definition SkipA ::
+"'VALUE ALPHABET \<Rightarrow> 'VALUE WF_ALPHA_PREDICATE" ("IID") is
+"\<lambda> a. (a \<union>\<^sub>f OK, true \<turnstile> II \<langle>a\<rangle>\<^sub>f)"
+  apply (auto simp add:WF_ALPHA_PREDICATE_def WF_PREDICATE_OVER_def DesignP_def)
+  apply (rule unrest)
+  apply (rule unrest)
+  apply (force intro:unrest)
+  apply (force intro:unrest)
+  apply (rule unrest)
+  apply (force intro:unrest)
+  apply (force intro:unrest)
+done
+*)
 
-definition H2 :: "('VALUE, 'TYPE) ALPHA_FUNCTION" where
-"H2 \<equiv> \<lambda> p. (p ;\<alpha> J (\<alpha> p))"
+declare DesignA_def [evala]
+declare SkipA_def [evala]
 
-definition H2' :: "('VALUE, 'TYPE) ALPHA_FUNCTION" where
-"H2' \<equiv> \<lambda> p. [p\<^sup>t \<Rightarrow>\<alpha> (p\<^sup>f)]\<alpha>"
+abbreviation is_healthy :: 
+  " 'VALUE WF_ALPHA_PREDICATE 
+  \<Rightarrow> 'VALUE ALPHA_FUNCTION 
+  \<Rightarrow> bool" ("_ is _ healthy") where
+"is_healthy p H \<equiv> p = H p"
 
-definition H3 :: "('VALUE, 'TYPE) ALPHA_FUNCTION" where
-"H3 \<equiv> \<lambda> p. p ;\<alpha> IID (\<alpha> p)"
+(*
+definition Mk_ALPHA_FUNCTION :: 
+  "'VALUE ALPHABET \<Rightarrow> 'VALUE WF_FUNCTION \<Rightarrow> 'VALUE ALPHA_FUNCTION" where
+"Mk_ALPHA_FUNCTION a f = (\<lambda> p. Abs_WF_ALPHA_PREDICATE (\<alpha> p, f (\<pi> p)))"
+*)
 
-definition H4 :: "('VALUE, 'TYPE) ALPHA_FUNCTION" where
-"H4 \<equiv> \<lambda> p. p ;\<alpha> true (\<alpha> p) \<Rightarrow>\<alpha> true (\<alpha> p)"
+definition "H1   \<equiv> \<lambda> p. ok \<Rightarrow>\<alpha> p"
+definition "J a  \<equiv> (ok \<Rightarrow>\<alpha> ok') \<and>\<alpha> II\<alpha> a"
+definition "H2   \<equiv> \<lambda> p. (p ;\<alpha> J (\<alpha> p))"
+(* definition "H2'  \<equiv> \<lambda> p. [p\<^sup>t \<Rightarrow>p (p\<^sup>f)]p" *)
+definition "H3  \<equiv> \<lambda> p. p ;\<alpha> IID (\<alpha> p)"
+definition "H4  \<equiv> \<lambda> p. p ;\<alpha> true (\<alpha> p) \<Rightarrow>\<alpha> true (\<alpha> p)"
 
+lemma extreme_point_true:
+  "false a \<turnstile> false a = false a \<turnstile> true a"
+  apply (utp_alpha_tac)
+  apply (utp_pred_tac)
+done
+
+(*
+lemma extreme_point_nok:
+  "true a \<turnstile> false a = \<not>\<alpha> ok"
+  apply (utp_alpha_tac)
+  apply (utp_pred_tac)
+  by (utp_pred_tac)
+*)
+
+lemma export_precondition:
+  "p \<turnstile> q = p \<turnstile> p \<and>\<alpha> q"
+  by (utp_alpha_tac, utp_pred_auto_tac)
+
+lemma BoolType_var_control_cases [elim]:
+  "\<lbrakk> type x = BoolType; \<not> control x \<Longrightarrow> P; \<langle>b\<rangle>\<^sub>b x = TrueV \<Longrightarrow> P; \<langle>b\<rangle>\<^sub>b x = FalseV \<Longrightarrow> P \<rbrakk> \<Longrightarrow> P"
+  by (metis MkBool_cases binding_value_alt var_compat_def)
+
+lemma EvalP_BoolType_cases [intro]:
+  "\<lbrakk> type x = BoolType; control x; \<lbrakk>p\<rbrakk>(b(x :=\<^sub>b TrueV)) ; \<lbrakk>p\<rbrakk>(b(x :=\<^sub>b FalseV)) \<rbrakk> \<Longrightarrow> \<lbrakk>p\<rbrakk>b"
+  by (metis (lifting) BoolType_var_control_cases binding_upd_simps(2))
+
+
+
+(*
+lemma "\<lbrakk> \<lbrakk>p\<rbrakk>b; \<And> x t. \<lbrakk> v : type x; \<D> v; \<lbrakk>p\<rbrakk>(b(x :=\<^sub>b v)) \<rbrakk> \<Longrightarrow> P \<rbrakk> \<Longrightarrow> P"
+  apply (simp add:EvalP_def)
+*)
+
+
+lemma BoolType_control_var_split:
+  "\<lbrakk> type x = BoolType; control x \<rbrakk> 
+  \<Longrightarrow> [p]\<alpha> = [p[FalseAE|x]\<alpha> \<and>\<alpha> p[TrueAE|x]\<alpha>]\<alpha>"
+  apply (subgoal_tac "\<lbrakk>TrueAE\<rbrakk>\<alpha>\<epsilon> \<rhd>\<^sub>e x")
+  apply (subgoal_tac "x \<notin> \<langle>\<alpha> TrueAE\<rangle>\<^sub>f")
+  apply (subgoal_tac "\<lbrakk>FalseAE\<rbrakk>\<alpha>\<epsilon> \<rhd>\<^sub>e x")
+  apply (subgoal_tac "x \<notin> \<langle>\<alpha> FalseAE\<rangle>\<^sub>f")
+  apply (rule EvalA_intro)
+  apply (simp add:alphabet)
+  apply (rule EvalP_intro)
+  apply (simp add:evala eval)
+  apply (utp_expr_tac)
+  apply (auto)[1]
+  apply (utp_alpha_tac)
+  apply (simp add:evala)
+  apply (force intro:defined typing)  
+  apply (utp_alpha_tac)
+  apply (simp add:evala)
+  apply (force intro:defined typing)  
+done
+
+lemma [evala]: "\<epsilon> e = \<lbrakk>e\<rbrakk>\<alpha>\<epsilon>"
+  by (simp add:EvalAE_def)
+
+lemma [evala]: 
+  "ok[false|okay]\<alpha> = FALSE" "ok[true|okay]\<alpha> = TRUE"
+  "ok'[false|okay']\<alpha> = FALSE" "ok'[true|okay']\<alpha> = TRUE"
+  by (auto simp add:eval evale evala alphabet)
+
+lemma [evala]: 
+  "ok[false|okay']\<alpha> = ok" "ok[true|okay']\<alpha> = ok"
+  "ok'[false|okay]\<alpha> = ok'" "ok'[true|okay]\<alpha> = ok'"
+  by (auto simp add:eval evale evala alphabet)
+
+lemma [simp]: "false \<and>p x = false" "false \<Rightarrow>p x = true" "p \<Rightarrow>p true = true" "true \<and>p p = p"
+  by (utp_pred_tac)+
+
+lemma DesignA_refinement:
+  assumes 
+    "PROGRAM_ALPHABET (\<alpha> p1)" "PROGRAM_ALPHABET (\<alpha> p2)"
+    "PROGRAM_ALPHABET (\<alpha> q1)" "PROGRAM_ALPHABET (\<alpha> q2)"
+  shows "(p1 \<turnstile> q1) \<sqsubseteq>\<alpha> (p2 \<turnstile> q2) = [p1 \<Rightarrow>\<alpha> p2]\<alpha> \<and>\<alpha> [p1 \<and>\<alpha> q2 \<Rightarrow>\<alpha> q1]\<alpha>"
+proof -
+  have "(p1 \<turnstile> q1) \<sqsubseteq>\<alpha> (p2 \<turnstile> q2) = [(p2 \<turnstile> q2) \<Rightarrow>\<alpha> (p1 \<turnstile> q1)]\<alpha>"
+    by (utp_alpha_tac, utp_pred_tac)
+
+  also have "... = [(ok \<and>\<alpha> p2 \<Rightarrow>\<alpha> ok' \<and>\<alpha> q2) \<Rightarrow>\<alpha> (ok \<and>\<alpha> p1 \<Rightarrow>\<alpha> ok' \<and>\<alpha> q1)]\<alpha>"
+    by (utp_alpha_tac)
+
+  also have "... = [(p2 \<Rightarrow>\<alpha> ok' \<and>\<alpha> q2) \<Rightarrow>\<alpha> (p1 \<Rightarrow>\<alpha> ok' \<and>\<alpha> q1)]\<alpha>"
+    apply (rule_tac trans)
+    apply (rule_tac x="okay" in BoolType_control_var_split)
+    apply (simp_all)
+    apply (simp add:SubstA_ImpliesA SubstA_AndA SubstA_OrA evala alphabet)
+    apply (insert assms)
+    apply (simp add:alphabet evala)
+  done
+
+  also have "... = [(\<not>\<alpha> p2 \<Rightarrow>\<alpha> \<not>\<alpha> p1) \<and>\<alpha> ((p2 \<Rightarrow>\<alpha> q2) \<Rightarrow>\<alpha> (p1 \<Rightarrow>\<alpha> q1))]\<alpha>"
+    apply (rule_tac trans)
+    apply (rule_tac x="okay'" in BoolType_control_var_split)
+    apply (simp_all)
+    apply (simp add:SubstA_ImpliesA SubstA_AndA SubstA_OrA evala alphabet)
+    apply (insert assms)
+    apply (simp add:alphabet evala eval)
+  done
+
+  also have "... = [(p1 \<Rightarrow>\<alpha> p2) \<and>\<alpha> ((p2 \<Rightarrow>\<alpha> q2) \<Rightarrow>\<alpha> (p1 \<Rightarrow>\<alpha> q1))]\<alpha>"
+    by (auto simp add:alphabet evala eval)
+
+  also have "... = [(p1 \<Rightarrow>\<alpha> p2)]\<alpha> \<and>\<alpha> [p1 \<and>\<alpha> q2 \<Rightarrow>\<alpha> q1]\<alpha>"
+    by (auto simp add:alphabet evala eval)
+
+  ultimately show ?thesis
+    by simp
+qed
+
+lemma DesignA_diverge:
+  "\<lbrakk> PROGRAM_ALPHABET (\<alpha> p); PROGRAM_ALPHABET (\<alpha> q) \<rbrakk> \<Longrightarrow>
+   (p \<turnstile> q)[false|okay]\<alpha> = true (\<alpha> p \<union>\<^sub>f \<alpha> q \<union>\<^sub>f (finsert okay' {}\<^sub>f))"
+  apply (simp add:DesignA_def)
+  apply (simp add:SubstA_ImpliesA SubstA_AndA evala alphabet)
+  apply (auto)
+done
+
+lemma H1_idempotent: "H1 (H1 p) = H1 p"
+  apply (simp add:H1_def)
+  apply (utp_alpha_tac)
+  apply (utp_pred_auto_tac)
+done
+
+lemma H1_DesignD: "p \<turnstile> q is H1 healthy"
+  apply (simp add:DesignA_def H1_def)
+  apply (utp_alpha_tac)
+  apply (utp_rel_auto_tac)
+done
+
+lemma J_split: "P ;\<alpha> J (\<alpha> P) = P\<^sup>f \<or>\<alpha> (P\<^sup>t \<and>\<alpha> ok')"
+  apply (simp add: J_def)
+  apply (utp_alpha_tac)
+  apply (utp_pred_auto_tac)
+oops
+
+lemma H2_H2': "P is H2 healthy \<longleftrightarrow> taut ([P\<^sup>t \<Rightarrow>p (P\<^sup>f)]p)"
+proof -
+  have "P is H2 healthy \<longleftrightarrow> P = P ; J"
+    by (simp add: H2_def)
+  
+  also have "... = 
+
+  apply (simp add:H2_def H2'_def J_def)
+  apply (utp_pred_auto_tac)
+  apply (utp_rel_auto_tac)
+
+lemma H2_idempotent: "H2 (H2 p) = H2 p"
+  apply (simp add:H2_def J_def)
+  apply (utp_rel_auto_tac)
+done
+
+lemma J_H2: "H2 J = J"
+  apply (simp add:H2_def J_def)
+  apply (utp_rel_auto_tac)
+done
+
+lemma H2_DesignD: "p \<turnstile> q is H2 healthy"
+  apply (simp add:DesignD_def H2_def J_def)
+  apply (utp_rel_auto_tac)
+  apply (auto simp add: EvalR_UNIV)
+
+lemma H1_H2_commute: "H1 (H2 p) = H2 (H1 p)"
+  apply (simp add:H1_def H2_def J_def)
+  apply (utp_rel_auto_tac)
+oops
+
+lemma H3_idempotent: "H3 (H3 p) = H3 p"
+  apply (simp add:H3_def SkipD_def DesignD_def)
+  apply (utp_rel_tac)
+  apply (auto)
+oops
+
+lemma H4_idempotent: "H4 (H4 p) = H4 p"
+  apply (simp add:H4_def)
+  apply (utp_rel_tac)
+  apply (auto)
+
+done
+
+
+(*
 definition DESIGN_ALPHABET :: "'TYPE ALPHABET set"
 where "DESIGN_ALPHABET = REL_ALPHABET \<inter> {a. OK \<subseteq> a}"
 
-(*
+
 {a. a \<in> WF_ALPHABET \<and> a \<subseteq> UNDASHED \<union> DASHED \<and> OK \<subseteq> a}"
 *)
 
@@ -305,6 +532,6 @@ lemma H1_design:
  (p \<turnstile> q) = H1 (p \<turnstile> q)"
   apply(simp add:DesignD_def H1_def)
   oops
+*)
 
-end
 end
