theories/utp_meta.thy
@@ -9,11 +9,10 @@ header {* Meta-Theory for Everything *}
 theory utp_meta
 imports
   utp_common
-  utp_global
   "core/utp_core"
   "alpha/utp_alpha"
-  "models/utp_models"
-  "models/utp_std_pred"
+(*  "models/utp_models"
+  "models/utp_std_pred" *)
   "tactics/utp_pred_tac"
   "tactics/utp_rel_tac"
   "tactics/utp_alpha_tac"
